Internal refinement (#53)
* redefine refines, ctx_refines as iProp

* fix libraries

* remove modc

theories/simulations/ctxrefine/CtxRefine.v
@@ -8,28 +8,36 @@ Definition refines_lmod (ms_tgt ms_src: LMod.t) : Prop :=
   Beh.of_itree (LMod.compile ms_tgt tt↑) <1=
   Beh.of_itree (LMod.compile ms_src tt↑).
 
-Section CTX_REFINE.
+Section REFINEMENT.
+
   Context `{!crisG Γ Σ α β τ _S _I}.
 
-  (* Definition of ctx refinement in Mod Level. *)
-  Definition refines (mpt : Mod.modc) (mps : Mod.modc) : Prop :=
-    let ms := mps.1 in let Ps := mps.2 in
-    let mt := mpt.1 in let Pt := mpt.2 in
+  Definition _refines (Mt Ms : Mod.t) : Σ -> Prop :=
+    fun r => Mod.wf Mt ->
+          Mod.wf Ms /\
+            forall rt rs,
+              (Own rs ⊢ Own rt ∗ Own r ∗ winv (∅,∅)) ->
+              ✓ rs -> refines_lmod (Mod.to_lmod Mt rt) (Mod.to_lmod Ms rs).
 
-    ∀ (WFM : Mod.wf mt),
-      Mod.wf ms /\
-      ∀ rs
-        (WFR : ✓ rs) (SRC : Own rs ⊢ |==> winv (∅,∅) ∗ Ps),
-        ∃ rt,
-          ✓ rt /\ (Own rt ⊢ |==> winv (∅,∅) ∗ Pt)%I /\
-          refines_lmod
-            (Mod.to_lmod mt rt)
-            (Mod.to_lmod ms rs).
+  Lemma _refines_mono Mt Ms
+    : ∀ (x1 x2 : Σ), _refines Mt Ms x1 → x1 ≼ x2 → _refines Mt Ms x2.
+  Proof.
+    unfold _refines.
+    intros x1 x2 M_LE x_LE WFT.
+    specialize (M_LE WFT). destruct M_LE as [WFS M_LE]. split; et.
+    intros rt rs SPLIT V. eapply M_LE; et.
+    iIntros "H".
+    iPoseProof (SPLIT with "H") as "($ & H & $)".
+    iApply Own_extends; et.
+  Qed.
 
-  Definition ctx_refines (mpt mps: Mod.modc) : Prop :=
-    ∀ (ctx : Mod.modc),
-      refines
-        (mpt.1 ★ ctx.1, mpt.2 ∗ ctx.2)%I
-        (mps.1 ★ ctx.1, mps.2 ∗ ctx.2)%I.
-End CTX_REFINE.
-Global Instance: Params (@ctx_refines) 1 := {}.
+  Definition refines_def (Mt Ms : Mod.t) : iProp Σ :=
+    {| uPred_holds := _refines Mt Ms; uPred_mono := _refines_mono Mt Ms |}.
+  Definition refines_aux : seal (@refines_def). Proof. by eexists. Qed.
+  Definition refines := refines_aux.(unseal).
+  Definition refines_unseal : @refines = @refines_def := refines_aux.(seal_eq).
+
+  Definition ctx_refines (Mt Ms : Mod.t) : iProp Σ :=
+    ∀ (Ctx : Mod.t), refines (Mt ★ Ctx) (Ms ★ Ctx).
+
+End REFINEMENT.
