library/apc/APCACproof.v
@@ -130,8 +130,8 @@ Section ctxr.
               ∧ (∀ X, msk _ (subevent _ (Choose X)) = true)
               ∧ (∀ X, msk _ (subevent _ (Assume X)) = true)
               ∧ (∀ X, msk _ (subevent _ (Guarantee X)) = true)) :
-    ctx_refines
-      ((APCA.t sp_pure sp_a)  ★ md, emp%I)
-      ((APCC.t sp_c)          ★ md, emp%I).
+    ⊢ ctx_refines
+      (APCA.t sp_pure sp_a ★ md)
+      (APCC.t sp_c ★ md).
   Proof. eapply main_adequacy, sim; eauto. Qed.
 End ctxr. End APCAC.
