library/helping/HelpingAux.v
@@ -31,111 +31,124 @@ Section props.
 
   Lemma gsim_option_Guarantee_both (N : option namespace)
       r g RR p_s p_t st_s st_t prog_s prog_t tid_s tid_t tp_s tp_t
-      scp k_s k_t (res : Σ) :
+      scp k_s k_t (res_t res_s : Σ) :
     tp_s !! tid_s =
       Some (⇓cris (x <- ⇓sb(msk_scp scp msk_true) (option_Guarantee N);; k_s x)) →
     tp_t !! tid_t =
       Some (⇓cris (x <- ⇓sb(msk_scp scp msk_true) (option_Guarantee N);; k_t x)) →
-    ✓ res →
-    (∀ (res1 : Σ), ✓ res1 →
+    ✓ res_s →
+    res_t ≼ res_s →
+    (∀ (res_t1 res_s1 : Σ), ✓ res_s1 → res_t1 ≼ res_s1 →
       gpaco7 _gsim (cpn7 _gsim) r g (lstateT * Any.t)%type (lstateT * Any.t)%type RR p_s p_t
         (LModTr.interp_stateE Any.t (iterV (LModTr.handle_callE prog_s)
           (tid_s, <[tid_s := ⇓cris (k_s tt)]> tp_s))
-          (st_s, (res1↑)))
+          (st_s, (res_s1↑)))
         (LModTr.interp_stateE Any.t (iterV (LModTr.handle_callE prog_t)
           (tid_t, <[tid_t := ⇓cris (k_t tt)]> tp_t))
-          (st_t, (res1↑)))) →
+          (st_t, (res_t1↑)))) →
     gpaco7 _gsim (cpn7 _gsim) r g (lstateT * Any.t)%type (lstateT * Any.t)%type RR p_s p_t
       (LModTr.interp_stateE Any.t
-        (iterV (LModTr.handle_callE prog_s) (tid_s, tp_s)) (st_s, (res↑)))
+        (iterV (LModTr.handle_callE prog_s) (tid_s, tp_s)) (st_s, (res_s↑)))
       (LModTr.interp_stateE Any.t
-        (iterV (LModTr.handle_callE prog_t) (tid_t, tp_t)) (st_t, (res↑))).
+        (iterV (LModTr.handle_callE prog_t) (tid_t, tp_t)) (st_t, (res_t↑))).
   Proof using.
-    intros Hin_s Hin_t Hres Hk.
+    intros Hin_s Hin_t Hres Hr Hk.
     eapply lookup_lt_Some in Hin_s as ?.
     eapply lookup_lt_Some in Hin_t as ?.
     destruct N as [N | ]; cycle 1.
     { ss; rewrite SBRed.ret ?bind_ret_l in Hin_s, Hin_t.
-      specialize (Hk res Hres); revert Hk; rewrite ?list_insert_id //=.
+      specialize (Hk res_t res_s Hres Hr); revert Hk.
+      rewrite ?list_insert_id //=.
     }
     eapply gsim_Guarantee_tgt; [rewrite Hin_t; do 2 f_equal; s; hnorm_itr|].
-    intros res2 Hres2. ghcNormT.
+    intros res_t1 [Hres_t1 Hupd].
     eapply gsim_Guarantee_src; [rewrite Hin_s; do 2 f_equal; s; hnorm_itr|].
-    exists res2; splits; try by des. ghcNormS.
-    eapply gsim_flag; last eapply (Hk res2).
-    { destruct p_s; rr; ss; eauto. }
-    { destruct p_t; rr; ss; eauto. }
-    by des.
+    exists res_t1; splits; try by des.
+    { iIntros "H". iPoseProof (Own_extends with "H") as "H"; et.
+      iApply Hupd. et.
+    }
+    ghcNormS; ghcNormT.
+    eapply gsim_flag; last eapply (Hk res_t1 res_t1); et.
+    - destruct p_s; rr; ss; eauto.
+    - destruct p_t; rr; ss; eauto.
   Qed.
 
   Lemma gsim_option_Assume_both (N : option namespace)
       r g RR p_s p_t st_s st_t prog_s prog_t tid_s tid_t tp_s tp_t
-      scp k_s k_t (res : Σ) :
+      scp k_s k_t (res_t res_s : Σ) :
     tp_s !! tid_s =
       Some (⇓cris (x <- ⇓sb(msk_scp scp msk_true) (option_Assume N);; k_s x)) →
     tp_t !! tid_t =
       Some (⇓cris (x <- ⇓sb(msk_scp scp msk_true) (option_Assume N);; k_t x)) →
-    ✓ res →
-    (∀ (res1 : Σ), ✓ res1 →
+    ✓ res_s →
+    res_t ≼ res_s →
+    (∀ (res_t1 res_s1 : Σ), ✓ res_s1 → res_t1 ≼ res_s1 →
       gpaco7 _gsim (cpn7 _gsim) r g (lstateT * Any.t)%type (lstateT * Any.t)%type RR p_s p_t
         (LModTr.interp_stateE Any.t (iterV (LModTr.handle_callE prog_s)
           (tid_s, <[tid_s := ⇓cris (k_s tt)]> tp_s))
-          (st_s, (res1↑)))
+          (st_s, (res_s1↑)))
         (LModTr.interp_stateE Any.t (iterV (LModTr.handle_callE prog_t)
           (tid_t, <[tid_t := ⇓cris (k_t tt)]> tp_t))
-          (st_t, (res1↑)))) →
+          (st_t, (res_t1↑)))) →
     gpaco7 _gsim (cpn7 _gsim) r g (lstateT * Any.t)%type (lstateT * Any.t)%type RR p_s p_t
       (LModTr.interp_stateE Any.t
-        (iterV (LModTr.handle_callE prog_s) (tid_s, tp_s)) (st_s, (res↑)))
+        (iterV (LModTr.handle_callE prog_s) (tid_s, tp_s)) (st_s, (res_s↑)))
       (LModTr.interp_stateE Any.t
-        (iterV (LModTr.handle_callE prog_t) (tid_t, tp_t)) (st_t, (res↑))).
+        (iterV (LModTr.handle_callE prog_t) (tid_t, tp_t)) (st_t, (res_t↑))).
   Proof using.
-    intros Hin_s Hin_t Hres Hk.
+    intros Hin_s Hin_t Hres Hr Hk.
     eapply lookup_lt_Some in Hin_s as ?.
     eapply lookup_lt_Some in Hin_t as ?.
     destruct N as [N | ]; cycle 1.
     { ss; rewrite SBRed.ret ?bind_ret_l in Hin_s, Hin_t.
-      specialize (Hk res Hres); revert Hk; rewrite ?list_insert_id //=.
+      specialize (Hk res_t res_s Hres Hr); revert Hk.
+      rewrite ?list_insert_id //=.
     }
     eapply gsim_Assume_src; [rewrite Hin_s; do 2 f_equal; s; hnorm_itr|].
-    intros res2 Hres2. ghcNormS.
+    intros res_s1 [Hres_s1 Hupd].
     eapply gsim_Assume_tgt; [rewrite Hin_t; do 2 f_equal; s; hnorm_itr|].
-    exists res2; splits; try by des. ghcNormT.
-    eapply gsim_flag; last eapply (Hk res2).
-    { destruct p_s; rr; ss; eauto. }
-    { destruct p_t; rr; ss; eauto. }
-    by des.
+    exists res_s1; splits; try by des.
+    { iIntros "H". iDestruct (Hupd with "H") as "> [$ H]".
+      iModIntro. iApply Own_extends; et.
+    }
+    ghcNormS; ghcNormT.
+    eapply gsim_flag; last eapply (Hk res_s1 res_s1); et.
+    - destruct p_s; rr; ss; eauto.
+    - destruct p_t; rr; ss; eauto.
   Qed.
 
   Lemma gsim_jobs_both
       (job : itree crisE (SAny.t + SAny.t))
       r g RR st_s st_t prog_s prog_t tid_s tid_t tp_s tp_t
-      sp k_s k_t (res : Σ) mn :
+      sp k_s k_t (res_t res_s : Σ) mn :
     tid_s < length tp_s →
     tid_t < length tp_t →
-    ✓ res →
-    (∀ (res1 : Σ) (ret : SAny.t + SAny.t), ✓ res1 →
+    ✓ res_s →
+    res_t ≼ res_s →
+    (∀ (res_t1 res_s1 : Σ) (ret : SAny.t + SAny.t),
+      ✓ res_s1 → res_t1 ≼ res_s1 →
       gpaco7 _gsim (cpn7 _gsim) r g (lstateT * Any.t)%type (lstateT * Any.t)%type RR smj_bot smj_bot
         (LModTr.interp_stateE Any.t (iterV (LModTr.handle_callE prog_s)
           (tid_s, <[tid_s := ⇓cris (k_s ret)]> tp_s))
-          (st_s, (res1↑)))
+          (st_s, (res_s1↑)))
         (LModTr.interp_stateE Any.t (iterV (LModTr.handle_callE prog_t)
           (tid_t, <[tid_t := ⇓cris (k_t ret)]> tp_t))
-          (st_t, (res1↑)))) →
+          (st_t, (res_t1↑)))) →
     gpaco7 _gsim (cpn7 _gsim) r g (lstateT * Any.t)%type (lstateT * Any.t)%type RR smj_bot smj_bot
       (LModTr.interp_stateE Any.t (iterV (LModTr.handle_callE prog_s) (tid_s,
         <[tid_s :=
           ⇓cris (x <- ⇓sb(msk_scp (HelpingOn.scopes mn) msk_true) (⇓smod(sp) (⇓sb(msk_pure) job));; k_s x)]>
-        tp_s)) (st_s, (res↑)))
+        tp_s)) (st_s, (res_s↑)))
       (LModTr.interp_stateE Any.t (iterV (LModTr.handle_callE prog_t) (tid_t,
         <[tid_t :=
           ⇓cris (x <- ⇓sb(msk_scp (HelpingOff.scopes mn) msk_true) (⇓smod(sp) (⇓sb(msk_pure) job));; k_t x)]>
-        tp_t)) (st_t, (res↑))).
+        tp_t)) (st_t, (res_t↑))).
   Proof using.
-    intros Hlen_s Hlen_t Hres Hk.
-    revert Hres Hk; generalize job res. clear job res.
+    intros Hlen_s Hlen_t Hres Hr Hk.
+    revert Hres Hr Hk; generalize job res_t res_s.
+    clear job res_t res_s.
     gcofix CIH.
-    intros job res Hres Hk.
+    intros job res_t res_s Hres Hr Hk.
     ides job.
     { ghcNormS; ghcNormT.
       eapply gpaco7_mon; eauto.
@@ -145,30 +158,44 @@ Section props.
       rewrite list_insert_insert.
       eapply gsim_tau_tgt; [rewrite list_lookup_insert //; do 2 f_equal; hnorm_itr|].
       rewrite list_insert_insert.
-      zprogress with smj_bot smj_bot _ _. gbase. eauto.
+      zprogress with smj_bot smj_bot _ _. gbase.
+      eapply CIH; eauto.
     }
     destruct e as [e|e]; rewrite !vis_trigger.
     { destruct e as [P|res1|P].
       { eapply gsim_Assume_src; [rewrite list_lookup_insert //; do 2 f_equal; hnorm_itr|].
-        intros res1 Hres1; rewrite list_insert_insert.
+        intros res_s1 [Hres_s1 Hupd]. rewrite list_insert_insert.
         eapply gsim_Assume_tgt; [rewrite list_lookup_insert //; do 2 f_equal; hnorm_itr|].
-        exists res1; splits; (try by des); rewrite list_insert_insert.
-        ghcNormS; ghcNormT.
-        zprogress with smj_bot smj_bot _ _. gbase. eapply CIH; try by des.
+        exists res_s1; splits; try by des.
+        { iIntros "H". iDestruct (Hupd with "H") as "> [$ H]".
+          iModIntro. iApply Own_extends; et.
+        }
+        rewrite list_insert_insert. ghcNormS; ghcNormT.
+        zprogress with smj_bot smj_bot _ _. gbase.
+        eapply CIH; try by des; et.
       }
       { eapply gsim_AssumeRes_src; [rewrite list_lookup_insert //; do 2 f_equal; hnorm_itr|].
-        intros ?; rewrite list_insert_insert.
+        intros Hres1; rewrite list_insert_insert.
         eapply gsim_AssumeRes_tgt; [rewrite list_lookup_insert //; do 2 f_equal; hnorm_itr|].
-        splits; (try by des); rewrite list_insert_insert.
-        ghcNormS; ghcNormT.
-        zprogress with smj_bot smj_bot _ _. gbase. eapply CIH; try by des.
+        splits.
+        { eapply cmra_valid_included; first eapply Hres1.
+          eapply cmra_mono_l; et.
+        }
+        rewrite list_insert_insert. ghcNormS; ghcNormT.
+        zprogress with smj_bot smj_bot _ _. gbase.
+        eapply CIH; try by des.
+        eapply cmra_mono_l; et.
       }
       { eapply gsim_Guarantee_tgt; [rewrite list_lookup_insert //; do 2 f_equal; hnorm_itr|].
-        intros res1 Hres1; rewrite list_insert_insert.
+        intros res_t1 [Hres_t1 Hupd]. rewrite list_insert_insert.
         eapply gsim_Guarantee_src; [rewrite list_lookup_insert //; do 2 f_equal; hnorm_itr|].
-        exists res1; splits; (try by des); rewrite list_insert_insert.
-        ghcNormS; ghcNormT.
-        zprogress with smj_bot smj_bot _ _. gbase. eapply CIH; try by des.
+        exists res_t1; splits; try by des.
+        { iIntros "H". iPoseProof (Own_extends with "H") as "H"; et.
+          iApply Hupd. et.
+        }
+        rewrite list_insert_insert. ghcNormS; ghcNormT.
+        zprogress with smj_bot smj_bot _ _. gbase.
+        eapply CIH; try by des; et.
       }
     }
     destruct e as [e|e].
@@ -186,20 +213,20 @@ Section props.
       eapply gsim_Choose_src; [rewrite list_lookup_insert //; do 2 f_equal; hnorm_itr|].
       exists x; rewrite list_insert_insert.
       ghcNormS; ghcNormT.
-      zprogress with smj_bot smj_bot _ _. gbase. eapply CIH; try by des.
+      zprogress with smj_bot smj_bot _ _. gbase. eapply CIH; eauto.
     }
     { eapply gsim_Take_src; [rewrite list_lookup_insert //; do 2 f_equal; hnorm_itr|].
       intros x; rewrite list_insert_insert.
       eapply gsim_Take_tgt; [rewrite list_lookup_insert //; do 2 f_equal; hnorm_itr|].
       exists x; rewrite list_insert_insert.
       ghcNormS; ghcNormT.
-      zprogress with smj_bot smj_bot _ _. gbase. eapply CIH; try by des.
+      zprogress with smj_bot smj_bot _ _. gbase. eapply CIH; eauto.
     }
     { giter_s; giter_t.
       rewrite /= ?list_lookup_insert //=. gcNormS; gcNormT.
       gstep_s. instantiate (1:=smj_top).
       intros ? ? <-. gsteps_s; gsteps_t. rewrite ?list_insert_insert. ired.
-      zprogress with smj_bot smj_bot _ _. gbase. eapply CIH; try by des.
+      zprogress with smj_bot smj_bot _ _. gbase. eapply CIH; eauto.
     }
   Qed.
 End props.
