library/helping/HelpingFacts.v
@@ -21,30 +21,37 @@ Section Helping.
     i; des; subst; s; rewrite string_length_app; nia.
   Qed.
 
-  Lemma helping_refines fns (mM : string → Mod.t) (mA mI ctx : Mod.t) (P1 P2 P : iProp Σ) jobs
-    (REF1: ∀ Q mn,
+  Lemma helping_refines fns (mM : string → Mod.t) (mA mI ctx : Mod.t) jobs
+    (DISJ: get_fids (dom (Mod.fnsems (mA ★ SchI.t ★ ctx))) ## fns) :
+    (∀ mn,
       refines
-        (CFilter.filter (Helping.exports mn) mI ★ CFilter.filter (Helping.exports mn ∪ fns) (SchI.t ★ ctx) ★ (HelpingDummy.t mn), Q)
-        (mM mn ★ CFilter.filter (Helping.exports mn ∪ fns) (SchI.t ★ ctx) ★ (HelpingOn.t mn jobs), (P1 ∗ Q)%I))
-    (REF2: ∀ Q mn,
+        (CFilter.filter (Helping.exports mn) mI ★
+          CFilter.filter (Helping.exports mn ∪ fns) (SchI.t ★ ctx) ★
+          HelpingDummy.t mn)
+        (mM mn ★
+          CFilter.filter (Helping.exports mn ∪ fns) (SchI.t ★ ctx) ★
+          HelpingOn.t mn jobs)) ∗
+    (∀ mn,
       refines
-        (mM mn ★ CFilter.filter (Helping.exports mn ∪ fns) (SchI.t ★ ctx) ★ HelpingOff.t mn jobs, Q)
-        (mA ★ CFilter.filter (Helping.exports mn ∪ fns) (SchI.t ★ ctx), (P2 ∗ Q)%I))
-    (DISJ: get_fids (dom (Mod.fnsems (mA ★ SchI.t ★ ctx))) ## fns)
-    :
+        (mM mn ★
+          CFilter.filter (Helping.exports mn ∪ fns) (SchI.t ★ ctx) ★
+          HelpingOff.t mn jobs)
+        (mA ★ CFilter.filter (Helping.exports mn ∪ fns) (SchI.t ★ ctx))) ⊢
     refines
-      (mI ★ CFilter.filter fns (SchI.t ★ ctx), P)
-      (mA ★ SchI.t ★ ctx, (P1 ∗ P2 ∗ P)%I).
-  Proof using.
+      (mI ★ CFilter.filter fns (SchI.t ★ ctx))
+      (mA ★ SchI.t ★ ctx).
+  Proof using H.
+    iIntros "[REF1 REF2]".
     set (mn := mname_long (S (max
       (maxlen (elements (get_fids (dom (Mod.fnsems (mA ★ mI ★ SchI.t ★ ctx))))))
       (maxlen (Mod.scopes (mA ★ mI ★ SchI.t ★ ctx)))))).
 
-    etrans.
-    { eapply ctxr_refines, (CFilter.intro_filter (Helping.exports mn)). }
+    iApply refines_trans. iSplitR "REF1 REF2".
+    { iApply ctxr_refines. iApply (CFilter.intro_filter (Helping.exports mn)). }
 
-    etrans.
-    { eapply CFilter.intro_module with (bl := Helping.exports mn) (mc := (HelpingDummy.t mn)); et.
+    iApply refines_trans. iSplitR "REF1 REF2".
+    { iApply (CFilter.intro_module (Helping.exports mn)
+        (mI ★ CFilter.filter fns (SchI.t ★ ctx)) (HelpingDummy.t mn)); et.
       { eapply helping_dummy_wf. }
       { intros ? a ->%elem_of_list_singleton. subst mn. eapply elem_of_maxlen in a.
         rewrite mname_long_length !Mod.maxlen_scopes_add in a. nia.
@@ -62,65 +69,145 @@ Section Helping.
       { set_solver+. }
     }
 
-    etrans.
-    { rewrite CFilter.filter_app -CFilter.filter_union -!assoc. apply REF1. }
-
-    etrans.
-    { eapply ctxr_refines.
-      rewrite CFilter.filter_app.
-      ctxr_drop. ctxr_rotate. ctxr_drop.
-      eapply helping_onoff_correct; et. set_solver.
+    iApply refines_trans. iSplitL "REF1".
+    { rewrite CFilter.filter_app -CFilter.filter_union -!assoc.
+      iApply ("REF1" $! mn).
     }
 
-    etrans.
-    { evar_at_last_2; [apply REF2|].
-      do 2 f_equal. rewrite !CFilter.filter_app -!assoc.
-      rewrite (comm _ (_ _ SchI.t)) assoc. refl.
+    iApply (refines_trans _
+      (mM mn ★ CFilter.filter (Helping.exports mn ∪ fns) (SchI.t ★ ctx) ★
+        HelpingOff.t mn jobs) _).
+    iSplitR "REF2".
+    { iApply ctxr_refines.
+      rewrite !CFilter.filter_app.
+      replace
+        (mM mn ★
+          (CFilter.filter (Helping.exports mn ∪ fns) SchI.t ★
+            CFilter.filter (Helping.exports mn ∪ fns) ctx) ★
+          HelpingOn.t mn jobs)
+        with
+        ((mM mn ★ CFilter.filter (Helping.exports mn ∪ fns) ctx) ★
+          (HelpingOn.t mn jobs ★
+            CFilter.filter (Helping.exports mn ∪ fns) SchI.t))
+        by mod_eq_solver.
+      replace
+        (mM mn ★
+          (CFilter.filter (Helping.exports mn ∪ fns) SchI.t ★
+            CFilter.filter (Helping.exports mn ∪ fns) ctx) ★
+          HelpingOff.t mn jobs)
+        with
+        ((mM mn ★ CFilter.filter (Helping.exports mn ∪ fns) ctx) ★
+          (HelpingOff.t mn jobs ★
+            CFilter.filter (Helping.exports mn ∪ fns) SchI.t))
+        by mod_eq_solver.
+      iApply ctxr_frameL.
+      iApply helping_onoff_correct. set_solver.
     }
 
-    etrans.
-    { eapply ctxr_refines.
-      ctxr_rotate. ctxr_drop. eapply CFilter.intro_filter.
+    iApply refines_trans. iSplitL "REF2".
+    { iApply ("REF2" $! mn).
     }
-    repeat erewrite <-CFilter.filter_app. rewrite (comm _ _ mA).
-    etrans.
-    { eapply CFilter.elim_filter.
+
+    iApply (refines_trans _
+      (CFilter.filter (Helping.exports mn ∪ fns) (mA ★ SchI.t ★ ctx)) _).
+    iSplitR.
+    { iApply ctxr_refines.
+      replace
+        (mA ★ CFilter.filter (Helping.exports mn ∪ fns) (SchI.t ★ ctx))
+        with
+        (CFilter.filter (Helping.exports mn ∪ fns) (SchI.t ★ ctx) ★ mA)
+        by mod_eq_solver.
+      replace
+        (CFilter.filter (Helping.exports mn ∪ fns) (mA ★ SchI.t ★ ctx))
+        with
+        (CFilter.filter (Helping.exports mn ∪ fns) (SchI.t ★ ctx) ★
+          CFilter.filter (Helping.exports mn ∪ fns) mA)
+        by (rewrite !CFilter.filter_app; mod_eq_solver).
+      iApply ctxr_frameL. iApply CFilter.intro_filter.
+    }
+    iApply CFilter.elim_filter.
       rewrite disjoint_union_r. split; et.
       intros i Hi1 Hi2. rewrite -elem_of_elements in Hi1; eapply elem_of_maxlen in Hi1.
       eapply helping_exports_long in Hi2. rewrite mname_long_length in Hi2.
       rewrite Mod.dom_fnsems_add maxlen_get_fids_union in Hi1.
       do 2 rewrite Mod.dom_fnsems_add maxlen_get_fids_union in Hi2. nia.
-    }
-
-    eapply ctxr_refines.
-    eapply ctxr_consequence. iIntros "[$ [$ $]]".
   Qed.
 
-  Lemma helping_main (mM : string → Mod.t) (mA mI mE : Mod.t) (P1 P2 : iProp Σ) jobs :
+  Lemma helping_main (mM : string → Mod.t) (mA mI mE : Mod.t) jobs :
     (∀ mn,
       ctx_refines
-        (CFilter.filter (Helping.exports mn) (mI ★ mE ★ SchI.t) ★ (HelpingDummy.t mn), emp%I)
-        (mM mn ★ CFilter.filter (Helping.exports mn) (mE ★ SchI.t) ★ (HelpingOn.t mn jobs), P1)) →
+        (CFilter.filter (Helping.exports mn) (mI ★ mE ★ SchI.t) ★
+          HelpingDummy.t mn)
+        (mM mn ★ CFilter.filter (Helping.exports mn) (mE ★ SchI.t) ★
+          HelpingOn.t mn jobs)) ∗
     (∀ mn,
-      (ctx_refines
-        (mM mn ★ CFilter.filter (Helping.exports mn) (mE ★ SchI.t) ★ HelpingOff.t mn jobs, emp%I))
-        (mA    ★ CFilter.filter (Helping.exports mn) (mE ★ SchI.t), P2)) →
+      ctx_refines
+        (mM mn ★ CFilter.filter (Helping.exports mn) (mE ★ SchI.t) ★
+          HelpingOff.t mn jobs)
+        (mA ★ CFilter.filter (Helping.exports mn) (mE ★ SchI.t))) ⊢
     ctx_refines
-      (mI ★ mE ★ SchI.t, emp%I)
-      (mA ★ mE ★ SchI.t, (P1 ∗ P2)%I).
+      (mI ★ mE ★ SchI.t)
+      (mA ★ mE ★ SchI.t).
   Proof.
-    intros REF1 REF2 [ctx P]; s.
-    rewrite (comm _ mE) -!assoc.
-    etrans; [|eapply helping_refines with (mI := mI) (mM := mM) (fns:=∅)]; cycle 1; i.
-    - rewrite CFilter.filter_union CFilter.filter_empty -{1}(left_id _ bi_sep Q).
-      evar_at_last_1; [evar_at_last_2|]; [eapply (REF1 _ (_,_))|..]; s.
-      + f_equal. rewrite !CFilter.filter_app. instantiate (1:= _ _ ctx). mod_eq_solver.
-      + f_equal. rewrite !CFilter.filter_app. mod_eq_solver.
-    - rewrite CFilter.filter_union CFilter.filter_empty -{1}(left_id _ bi_sep Q).
-      evar_at_last_1; [evar_at_last_2|]; [eapply (REF2 _ (_,_))|..]; s.
-      + f_equal. rewrite !CFilter.filter_app. instantiate (1:= _ _ ctx). mod_eq_solver.
-      + f_equal. rewrite !CFilter.filter_app. mod_eq_solver.
+    iIntros "[REF1 REF2]" (ctx).
+    replace
+      ((mI ★ mE ★ SchI.t) ★ ctx)
+      with
+      (mI ★ (SchI.t ★ (mE ★ ctx)))
+      by (rewrite !assoc;
+          rewrite -(assoc _ mI mE SchI.t) (comm _ mE SchI.t);
+          rewrite (assoc _ mI SchI.t mE); et).
+    rewrite -(CFilter.filter_empty (SchI.t ★ (mE ★ ctx))).
+    replace
+      ((mA ★ mE ★ SchI.t) ★ ctx)
+      with
+      (mA ★ SchI.t ★ (mE ★ ctx))
+      by (rewrite !assoc;
+          rewrite -(assoc _ mA mE SchI.t) (comm _ mE SchI.t);
+          rewrite (assoc _ mA SchI.t mE); et).
+    iApply (helping_refines ∅ mM mA mI (mE ★ ctx) jobs).
     - apply disjoint_empty_r.
-    - rewrite CFilter.filter_empty left_id. refl.
+    - iSplitL "REF1".
+      + iIntros (mn). iApply ctxr_refines.
+        replace (Helping.exports mn ∪ ∅) with (Helping.exports mn)
+          by set_solver.
+        replace
+          (CFilter.filter (Helping.exports mn) mI ★
+            CFilter.filter (Helping.exports mn) (SchI.t ★ (mE ★ ctx)) ★
+            HelpingDummy.t mn)
+          with
+          ((CFilter.filter (Helping.exports mn) (mI ★ mE ★ SchI.t) ★
+              HelpingDummy.t mn) ★
+            CFilter.filter (Helping.exports mn) ctx)
+          by (rewrite !CFilter.filter_app; mod_eq_solver).
+        replace
+          (mM mn ★
+            CFilter.filter (Helping.exports mn) (SchI.t ★ (mE ★ ctx)) ★
+            HelpingOn.t mn jobs)
+          with
+          ((mM mn ★ CFilter.filter (Helping.exports mn) (mE ★ SchI.t) ★
+              HelpingOn.t mn jobs) ★
+            CFilter.filter (Helping.exports mn) ctx)
+          by (rewrite !CFilter.filter_app; mod_eq_solver).
+        iApply ctxr_frameR. iApply ("REF1" $! mn).
+      + iIntros (mn). iApply ctxr_refines.
+        replace (Helping.exports mn ∪ ∅) with (Helping.exports mn)
+          by set_solver.
+        replace
+          (mM mn ★
+            CFilter.filter (Helping.exports mn) (SchI.t ★ (mE ★ ctx)) ★
+            HelpingOff.t mn jobs)
+          with
+          ((mM mn ★ CFilter.filter (Helping.exports mn) (mE ★ SchI.t) ★
+              HelpingOff.t mn jobs) ★
+            CFilter.filter (Helping.exports mn) ctx)
+          by (rewrite !CFilter.filter_app; mod_eq_solver).
+        replace
+          (mA ★ CFilter.filter (Helping.exports mn) (SchI.t ★ (mE ★ ctx)))
+          with
+          ((mA ★ CFilter.filter (Helping.exports mn) (mE ★ SchI.t)) ★
+            CFilter.filter (Helping.exports mn) ctx)
+          by (rewrite !CFilter.filter_app; mod_eq_solver).
+        iApply ctxr_frameR. iApply ("REF2" $! mn).
   Qed.
 End Helping.
