library/prophecy/ProphecyFacts.v
@@ -16,29 +16,39 @@ Section prophecy.
     i; des; subst; s; rewrite string_length_app; nia.
   Qed.
 
-  Lemma prophecy_refines sz (mds mdt ctx : Mod.t) (mdm : string → Mod.t) (Pm Ps : iProp Σ)
-    (REF1: ∀ Q,
-      refines
-        (CFilter.filter (Prophecy.exports (mname_long sz)) mdt ★ ProphecyI.t (mname_long sz) ★ CFilter.filter (Prophecy.exports (mname_long sz)) ctx, Q)
-        (mdm (mname_long sz) ★ ProphecyI.t (mname_long sz) ★ CFilter.filter (Prophecy.exports (mname_long sz)) ctx, (Pm ∗ Q)%I))
-    (REF2: ∀ Q,
-      refines
-        (mdm (mname_long sz) ★ ProphecyA.t (mname_long sz) ∅ ★ CFilter.filter (Prophecy.exports (mname_long sz)) ctx, Q)
-        (mds ★ CFilter.filter (Prophecy.exports (mname_long sz)) ctx, (Ps ∗ Q)%I))
-    (SZ: sz > max (maxlen (elements (get_fids (dom (Mod.fnsems (mds ★ mdt ★ ctx))))))
+  Lemma prophecy_refines sz (mds mdt ctx : Mod.t)
+      (mdm : string → Mod.t)
+    (SZ: sz > max (maxlen (elements (get_fids (dom
+                  (Mod.fnsems (mds ★ mdt ★ ctx))))))
                   (maxlen (Mod.scopes (mds ★ mdt ★ ctx))))
     (Realmdm: real_mod (mdm (mname_long sz)))
     (Realctx: real_mod ctx)
     :
     refines
-      (mdt ★ ctx, emp%I)
-      (mds ★ ctx, Pm ∗ ProphecyA.initial_cond ∗ Ps)%I.
+        (CFilter.filter (Prophecy.exports (mname_long sz)) mdt ★
+          ProphecyI.t (mname_long sz) ★
+          CFilter.filter (Prophecy.exports (mname_long sz)) ctx)
+        (mdm (mname_long sz) ★ ProphecyI.t (mname_long sz) ★
+          CFilter.filter (Prophecy.exports (mname_long sz)) ctx) ∗
+      ProphecyA.initial_cond ∗
+      refines
+        (mdm (mname_long sz) ★ ProphecyA.t (mname_long sz) ∅ ★
+          CFilter.filter (Prophecy.exports (mname_long sz)) ctx)
+        (mds ★
+          CFilter.filter (Prophecy.exports (mname_long sz)) ctx) ⊢
+      refines (mdt ★ ctx) (mds ★ ctx).
   Proof.
-    etrans.
-    { eapply ctxr_refines, (CFilter.intro_filter (Prophecy.exports (mname_long sz))). }
+    iIntros "[REF1 [INIT REF2]]".
+    iApply refines_trans. iSplitR "REF1 INIT REF2".
+    { iApply ctxr_refines.
+      iApply (CFilter.intro_filter
+        (Prophecy.exports (mname_long sz))).
+    }
 
-    etrans.
-    { eapply CFilter.intro_module with (mc := ProphecyI.t (mname_long sz)).
+    iApply refines_trans. iSplitR "REF1 INIT REF2".
+    { iApply (CFilter.intro_module
+        (Prophecy.exports (mname_long sz)) (mdt ★ ctx)
+        (ProphecyI.t (mname_long sz))).
       { econs; [mod_tac|prove_nodup]. }
       { set_solver. }
       { intros i Hi1 Hi2; rewrite -elem_of_elements in Hi1; eapply elem_of_maxlen in Hi1.
@@ -49,53 +59,67 @@ Section prophecy.
       { set_solver+. }
     }
     rewrite CFilter.filter_app.
-    etrans.
-    { rewrite -assoc (comm _ _ (ProphecyI.t _)). apply REF1. }
-    etrans.
-    { rewrite (comm _ (ProphecyI.t _)) assoc.
-      eapply ProphIA.adequacy_refines; eauto.
-      eapply real_mod_add; eauto using CFilter.real_mod.
+    iApply refines_trans. iSplitL "REF1".
+    { rewrite -assoc (comm _ _ (ProphecyI.t _)).
+      iExact "REF1".
     }
-    etrans.
-    { rewrite -assoc (comm _ _ (ProphecyA.t _ _)). apply REF2. }
-    etrans.
-    { eapply ctxr_refines. ctxr_rotate. ctxr_drop.
-      eapply CFilter.intro_filter. }
-    erewrite <-!CFilter.filter_app. ctxr_norm.
-    etrans.
-    { eapply CFilter.elim_filter.
+    iApply refines_trans. iSplitL "INIT".
+    { rewrite (comm _ (ProphecyI.t _)) assoc.
+      iApply ProphIA.adequacy_refines.
+      eapply real_mod_add; eauto using CFilter.real_mod.
+      done.
+    }
+    iApply refines_trans. iSplitL "REF2".
+    { rewrite -assoc (comm _ _ (ProphecyA.t _ _)).
+      iExact "REF2".
+    }
+    iApply refines_trans. iSplitR.
+    { iApply ctxr_refines. iApply ctxr_frameR.
+      iApply CFilter.intro_filter.
+    }
+    erewrite <-!CFilter.filter_app.
+    { iApply CFilter.elim_filter.
       intros i Hi1 Hi2; rewrite -elem_of_elements in Hi1; eapply elem_of_maxlen in Hi1.
       rewrite Mod.dom_fnsems_add maxlen_get_fids_union in Hi1.
       eapply prophecy_exports_long in Hi2. rewrite mname_long_length in Hi2.
       do 2 rewrite Mod.dom_fnsems_add maxlen_get_fids_union in SZ. nia.
     }
-
-    rewrite comm.
-    eapply ctxr_refines, ctxr_consequence; iIntros "[$ [$ $]]".
   Qed.
 
-  Lemma prophecy_main (mds mdt ctx : Mod.t) (mdm : string → Mod.t) (Pm Ps : iProp Σ) :
-    (∀ mn,
-      ctx_refines
-        (CFilter.filter (Prophecy.exports mn) mdt ★ ProphecyI.t mn, emp%I)
-        (mdm mn ★ ProphecyI.t mn, Pm)) →
-    (∀ mn,
-      ctx_refines
-        (mdm mn ★ ProphecyA.t mn ∅, emp%I)
-        (mds, Ps)) →
+  Lemma prophecy_main (mds mdt ctx : Mod.t) (mdm : string → Mod.t) :
     (∀ mn, real_mod (mdm mn)) →
     real_mod ctx →
-    refines (mdt ★ ctx, emp%I) (mds ★ ctx, Pm ∗ ProphecyA.initial_cond ∗ Ps)%I.
+    (∀ mn,
+      ctx_refines
+        (CFilter.filter (Prophecy.exports mn) mdt ★ ProphecyI.t mn)
+        (mdm mn ★ ProphecyI.t mn)) ∗
+      ProphecyA.initial_cond ∗
+      (∀ mn,
+      ctx_refines
+        (mdm mn ★ ProphecyA.t mn ∅)
+        mds) ⊢
+      refines (mdt ★ ctx) (mds ★ ctx).
   Proof.
-    intros REF1 REF2 Rmdm Rctx; s.
+    intros Rmdm Rctx; s.
     set (sz := S (max
                  (maxlen (elements (get_fids (dom (Mod.fnsems (mds ★ mdt ★ ctx))))))
                  (maxlen (Mod.scopes (mds ★ mdt ★ ctx))))).
-    eapply prophecy_refines with (sz:=sz); i; eauto using prophecy_exports_long; try nia.
-    - eapply ctxr_refines. rewrite !assoc -{1}(left_id _ bi_sep Q).
-      eapply ctxr_frameR, ctxr_cond_frameR. eapply REF1.
-    - eapply ctxr_refines. rewrite !assoc -{1}(left_id _ bi_sep Q).
-      eapply ctxr_frameR, ctxr_cond_frameR. eapply REF2.
+    iIntros "[REF1 [INIT REF2]]".
+    iApply (prophecy_refines sz mds mdt ctx mdm); try nia; eauto.
+    iSplitL "REF1".
+    - iApply ctxr_refines. rewrite !assoc.
+      iApply (ctxr_frameR
+        (CFilter.filter (Prophecy.exports (mname_long sz)) mdt ★
+          ProphecyI.t (mname_long sz))
+        (mdm (mname_long sz) ★ ProphecyI.t (mname_long sz))
+        (CFilter.filter (Prophecy.exports (mname_long sz)) ctx)).
+      iSpecialize ("REF1" $! (mname_long sz)). done.
+    - iFrame "INIT". iApply ctxr_refines. rewrite !assoc.
+      iApply (ctxr_frameR
+        (mdm (mname_long sz) ★ ProphecyA.t (mname_long sz) ∅)
+        mds
+        (CFilter.filter (Prophecy.exports (mname_long sz)) ctx)).
+      iSpecialize ("REF2" $! (mname_long sz)). done.
   Qed.
 
 End prophecy.
