theories/cancellation/MInlineElim.v
@@ -8,9 +8,10 @@ From stdpp Require Import base list.
 Section INLINE.
 Context `{!crisG Γ Σ α β τ _S _I}.
 
-Lemma inline_elim md P : refines (MInline.inline md, P) (md, P).
+Lemma inline_elim md :
+  ⊢ refines (MInline.inline md) md.
 Proof using.
-  eapply closed_adequacy_emp with (Ist:=IstEq). clear P.
+  eapply closed_adequacy with (Ist := IstEq).
 
   cut (∀ (f: emask * fbody) (WF: Mod.wf md) (SCP: ∀ X (e: crisE X), f.1 _ (subevent _ e) → (msk_scp (Mod.scopes md) msk_true) _ (subevent _ e)),
   isim_fsem
