theories/simulations/ctxrefine/ClosedAdequacy.v
@@ -10,35 +10,21 @@ From CRIS.simulations.ctxrefine Require Import CtxRefine.
 Section ADEQUACY.
   Context `{!crisG Γ Σ α β τ _S _I}.
 
-  Theorem closed_adequacy (ms mt : Mod.t) IC Ist P :
-    ISim.t closed ms mt IC Ist →
-    refines (mt, P) (ms, IC ∗ P)%I.
-  Proof using.
-    split.
-    { eapply ISim_wf; eauto. }
-    intros rs Hrsval [rwinv [ric [Hrs [Hrwinv Hric]]]]%Own_bupd_split; ss; eauto.
-    (* ii. ss. eapply Own_bupd_split in SRC; eauto. des. *)
-    eapply Own_split in Hric as [ric1 [ric2 [Hric [Hric1 Hric2]]]]; eauto; cycle 1.
-    { eapply Own_wand_valid, Hrsval. rewrite Hrs. iIntros ">[_ ?] //". }
-    rewrite winv_split_empty in Hrwinv.
-    eapply Own_split in Hrwinv as [rwinv1 [rwinv2 [Hrwinv [Hrwinv1 Hrwinv2]]]]; eauto; des; cycle 1.
-    { eapply Own_wand_valid, Hrsval. rewrite Hrs. iIntros ">[$ ?] //". }
-    exists (ric2 ⋅ rwinv2).
-    esplits; eauto.
-    { eapply Own_wand_valid, Hrsval. rewrite Hrs Hric Hrwinv !Own_op. iIntros ">[[? $] [? $]] //". }
-    { rewrite Own_op Hrwinv2 Hric2 comm; eauto. }
-    ii. eapply lsim_adequacy, PR.
-    - eapply ISim_adequacy; et.
-      rewrite Hrs Hric Own_op Hric1 Hrwinv !Own_op Hrwinv1.
-      iIntros ">[[? ?] [? ?]]". iFrame. eauto.
+  Theorem closed_adequacy (Mt Ms : Mod.t) IC Ist :
+    ISim.t closed Ms Mt IC Ist ->
+    IC ⊢ refines Mt Ms.
+  Proof.
+    intros SIM.
+    eapply entails_pointwise. intros x _ x_IC.
+    eapply Own_general_completeness.
+    rewrite refines_unseal /refines_def. change (_refines Mt Ms x).
+    intros WF. split. { eapply ISim_wf; et. }
+    intros rt rs SPLIT VALID.
+    unfold refines_lmod. eapply lsim_adequacy.
+    eapply ISim_adequacy; et.
+    iIntros "H". iModIntro.
+    iDestruct (SPLIT with "H") as "($ & H & $)".
+    iApply x_IC. done.
   Qed.
 
-  Theorem closed_adequacy_emp (ms mt : Mod.t) Ist P :
-    ISim.t closed ms mt emp%I Ist →
-    refines (mt, P) (ms, P).
-  Proof using.
-    intros Hsim%(closed_adequacy ms mt _ _ P).
-    ii. exploit Hsim; eauto. i; des. esplits; eauto.
-    i. exploit x1; eauto. ss. rewrite -bi.emp_sep_1. eauto.
-  Qed.
 End ADEQUACY.
